...

theories/FormalTerm.v
@@ -1,14 +1,18 @@
+From mathcomp Require Import ssreflect.
+Set Bullet Behavior "Strict Subproofs".
+
 Require Import Unicode.Utf8.
 Require Import Coq.Vectors.Vector.
+Require Import Coq.Program.Equality.
+Require Import Coq.omega.Omega.
 From gctt Require Import Terms.
 From gctt Require Import Axioms.
+From gctt Require Import GCTT.
+
 
 Set Implicit Arguments.
 
 Module FTm.
-  Inductive clk l :=
-  | cref : ∀ k, k < l → clk l.
-
   Inductive t (l n : nat) :=
   | var : forall i, i < n -> t l n
   | fst : t l n -> t l n
@@ -21,21 +25,58 @@ Module FTm.
   | prod : t l n -> t l n -> t l n
   | arr : t l n -> t l n -> t l n
   | pair : t l n -> t l n -> t l n
-  | ltr : clk l → t l n -> t l n
+  | ltr : Fin.t l → t l n -> t l n
   | isect : t (S l) n -> t l n
   | univ : nat -> t l n.
+
+
+  Fixpoint liftVar n (x : Fin.t n) : Fin.t (pred n) -> Fin.t n :=
+    match x with
+    | Fin.F1 _ => fun y => Fin.FS y
+    | Fin.FS _ x' => fun y =>
+                    match y in Fin.t n' return Fin.t n' -> (Fin.t (pred n') -> Fin.t n')
+                                             -> Fin.t (S n') with
+                    | Fin.F1 _ => fun x' _ => Fin.F1
+                    | Fin.FS _ y' => fun _ fx' => Fin.FS (fx' y')
+                    end x' (liftVar x')
+    end.
+
+  Fixpoint liftFin n (x : Fin.t n) : Fin.t (pred n) -> Fin.t n :=
+    match x with
+    | Fin.F1 _ => fun y => Fin.FS y
+    | Fin.FS _ x' =>
+      fun y =>
+        match y in Fin.t n' return Fin.t n' -> (Fin.t (pred n') -> Fin.t n') -> Fin.t (S n') with
+        | Fin.F1 _ => fun x' _ => Fin.F1
+        | Fin.FS _ y' => fun _ fx' => Fin.FS (fx' y')
+        end x' (liftFin x')
+    end.
+
+  Fixpoint kliftTm {l n} (e : t l n) (k : Fin.t (S l)) : t (S l) n :=
+    match e with
+    | var _ p => var _ p
+    | fst e => fst (kliftTm e k)
+    | snd e => snd (kliftTm e k)
+    | unit => unit _ _
+    | bool => bool _ _
+    | ax => ax _ _
+    | tt => tt _ _
+    | ff => ff _ _
+    | prod a b => prod (kliftTm a k) (kliftTm b k)
+    | arr a b => arr (kliftTm a k) (kliftTm b k)
+    | pair a b => pair (kliftTm a k) (kliftTm b k)
+    | ltr k' a => ltr (liftVar k k') (kliftTm a k)
+    | isect a => isect (kliftTm a (Fin.FS k))
+    | univ i => univ _ _ i
+    end.
+
+  Definition kwkTm {l n} (e : t l n) : t (S l) n :=
+    kliftTm e Fin.F1.
 End FTm.
 
 Definition Env := Vector.t CLK.
 
-
-Definition interp_clk {l : nat} (k : FTm.clk l) (ρ : Env l) : CLK :=
-  match k with
-  | FTm.cref _ p => Vector.nth_order ρ p
-  end.
-
 Reserved Notation "⟦ e ⟧ ρ" (at level 50).
-Notation "K⟦ k ⟧ ρ" := (interp_clk k ρ) (at level 50).
 Notation "κ ∷ ρ" := (Vector.cons _ κ _ ρ) (at level 30).
 
 Fixpoint interp {l n : nat} (e : FTm.t l n) (ρ : Env l) : Tm.t n :=
@@ -51,8 +92,68 @@ Fixpoint interp {l n : nat} (e : FTm.t l n) (ρ : Env l) : Tm.t n :=
   | FTm.prod A B => Tm.prod (⟦A⟧ ρ) (⟦B⟧ ρ)
   | FTm.arr A B => Tm.arr (⟦A⟧ ρ) (⟦B⟧ ρ)
   | FTm.pair A B => Tm.pair (⟦A⟧ ρ) (⟦B⟧ ρ)
-  | FTm.ltr ref A => Tm.ltr (K⟦ref⟧ ρ) (⟦A⟧ ρ)
+  | FTm.ltr r A => Tm.ltr (nth ρ r) (⟦A⟧ ρ)
   | FTm.isect A => Tm.isect (fun κ => ⟦A⟧ (κ ∷ ρ))
   | FTm.univ i => Tm.univ i
   end
 where "⟦ e ⟧ ρ" := (interp e ρ).
+
+Module Jdg.
+  Inductive atomic l n :=
+  | eq_ty : FTm.t l n → FTm.t l n → atomic l n.
+
+  Reserved Notation "J⟦ J ⟧" (at level 50).
+
+  Import Univ.
+
+  Definition meaning (l : nat) (J : atomic l 0) : Prop :=
+    match J with
+    | eq_ty A B =>
+      ∀ (ρ : Env l),
+        ⊧ ⟦ A ⟧ ρ ∼ ⟦ B ⟧ ρ
+    end.
+
+  Notation "⟦ n ∣ J ⟧" := (@meaning n J) (at level 50).
+
+  Lemma test :
+    ∀ l n (e : FTm.t l n) (ρ : Env (S l)),
+      ⟦ FTm.isect (FTm.kwkTm (FTm.ltr Fin.F1 (FTm.tt _ n))) ⟧ ρ
+      =
+      Tm.isect (fun κ => Tm.ltr (nth ρ Fin.F1) Tm.tt).
+  Proof.
+    move=> l n e ρ.
+    simpl.
+    auto.
+  Qed.
+
+
+  (* This should be true, just a little gnarly to prove. *)
+  Lemma interp_clk_wk :
+    ∀ l n (e : FTm.t l n) (ρ : Env l) (κ : CLK),
+      ⟦ e ⟧ ρ = ⟦ FTm.kwkTm e ⟧ (κ ∷ ρ).
+  Proof.
+  Admitted.
+
+
+  Theorem test3 :
+    ∀ (l : nat) (A : FTm.t l 0),
+      ⟦ l ∣ eq_ty A A ⟧
+      → ⟦ l ∣ eq_ty A (FTm.isect (FTm.kwkTm A)) ⟧.
+  Proof.
+    move=> l A D ρ.
+    simpl.
+    have : (λ κ : CLK, ⟦ FTm.kwkTm A ⟧ κ ∷ ρ) = (fun κ => ⟦A⟧ ρ).
+    + T.eqcd => κ.
+      by [rewrite -interp_clk_wk].
+    + move=> Q.
+      rewrite Q.
+      simpl.
+      apply: ClosedRules.isect_irrelevance.
+      simpl in D.
+      specialize (D ρ).
+      case: D => R [D1 D2].
+      eauto.
+  Qed.
+
+
+End Jdg.
